Source/Dafny/Translator.cs
@@ -6605,7 +6605,7 @@ namespace Microsoft.Dafny {
         return CanCallAssumption(e.E, etran);
       } else if (expr is OldExpr) {
         var e = (OldExpr)expr;
-        return CanCallAssumption(e.E, e.AtLabel == null ? etran.Old : etran.OldAt(e.AtLabel));
+        return CanCallAssumption(e.E, etran.OldAt(e.AtLabel));
       } else if (expr is UnchangedExpr) {
         var e = (UnchangedExpr)expr;
         Bpl.Expr be = Bpl.Expr.True;
@@ -7302,12 +7302,6 @@ namespace Microsoft.Dafny {
           } else {
             CheckNonNull(expr.tok, e.Obj, builder, etran, options.AssertKv);
             // Check that the receiver is available in the state in which the dereference occurs
-            if (etran.UsesOldHeap) {
-              Bpl.Expr wh = GetWhereClause(expr.tok, etran.TrExpr(e.Obj), e.Obj.Type, etran, ISALLOC, true);
-              if (wh != null) {
-                builder.Add(Assert(expr.tok, wh, "receiver must be allocated in the state in which its fields are accessed"));
-              }
-            }
           }
         } else if (e.Member is DatatypeDestructor) {
           var dtor = (DatatypeDestructor)e.Member;
@@ -7319,6 +7313,19 @@ namespace Microsoft.Dafny {
           } else {
             builder.Add(Assert(expr.tok, correctConstructor,
               string.Format("destructor '{0}' can only be applied to datatype values constructed by {1}", dtor.Name, dtor.EnclosingCtorNames("or"))));
+          }
+        }
+        if (!e.Member.IsStatic) {
+          if (e.Member is TwoStateFunction) {
+            Bpl.Expr wh = GetWhereClause(expr.tok, etran.TrExpr(e.Obj), e.Obj.Type, etran.OldAt(e.AtLabel), ISALLOC, true);
+            if (wh != null) {
+              builder.Add(Assert(expr.tok, wh, "receiver argument must be allocated in the two-state function's previous state"));
+            }
+          } else if (etran.UsesOldHeap) {
+            Bpl.Expr wh = GetWhereClause(expr.tok, etran.TrExpr(e.Obj), e.Obj.Type, etran, ISALLOC, true);
+            if (wh != null) {
+              builder.Add(Assert(expr.tok, wh, $"receiver must be allocated in the state in which its {(e.Member is Field ? "fields" : "members")} are accessed"));
+            }
           }
         }
         if (options.DoReadsChecks && e.Member is Field && ((Field)e.Member).IsMutable) {
@@ -7591,9 +7598,9 @@ namespace Microsoft.Dafny {
             }
           } else if (e.Function is TwoStateFunction) {
             if (!e.Function.IsStatic) {
-              Bpl.Expr wh = GetWhereClause(e.Receiver.tok, etran.TrExpr(e.Receiver), e.Receiver.Type, etran.Old, ISALLOC, true);
+              Bpl.Expr wh = GetWhereClause(e.Receiver.tok, etran.TrExpr(e.Receiver), e.Receiver.Type, etran.OldAt(e.AtLabel), ISALLOC, true);
               if (wh != null) {
-                builder.Add(Assert(e.Receiver.tok, wh, "receiver argument must be allocated in the two-state functions's previous state"));
+                builder.Add(Assert(e.Receiver.tok, wh, "receiver argument must be allocated in the two-state function's previous state"));
               }
             }
             Contract.Assert(e.Function.Formals.Count == e.Args.Count);
@@ -7601,7 +7608,7 @@ namespace Microsoft.Dafny {
               var formal = e.Function.Formals[i];
               if (formal.IsOld) {
                 Expression ee = e.Args[i];
-                Bpl.Expr wh = GetWhereClause(ee.tok, etran.TrExpr(ee), ee.Type, etran.Old, ISALLOC, true);
+                Bpl.Expr wh = GetWhereClause(ee.tok, etran.TrExpr(ee), ee.Type, etran.OldAt(e.AtLabel), ISALLOC, true);
                 if (wh != null) {
                   builder.Add(Assert(ee.tok, wh, string.Format("argument{0} ('{1}') must be allocated in the two-state function's previous state",
                     e.Args.Count == 1 ? "" : " " + i, formal.Name)));
@@ -7731,7 +7738,7 @@ namespace Microsoft.Dafny {
         // Anything read inside the 'old' expressions depends only on the old heap, which isn't included in the
         // frame axiom.  In other words, 'old' expressions have no dependencies on the current heap.  Therefore,
         // we turn off any reads checks for "e.E".
-        CheckWellformed(e.E, new WFOptions(options), locals, builder, e.AtLabel == null ? etran.Old : etran.OldAt(e.AtLabel));
+        CheckWellformed(e.E, new WFOptions(options), locals, builder, etran.OldAt(e.AtLabel));
       } else if (expr is UnchangedExpr) {
         var e = (UnchangedExpr)expr;
         foreach (var fe in e.Frame) {
@@ -8506,12 +8513,7 @@ namespace Microsoft.Dafny {
 
 
     void CheckFunctionSelectWF(string what, BoogieStmtListBuilder builder, ExpressionTranslator etran, Expression e, string hint) {
-      Function fn = null;
-      var sel = e as MemberSelectExpr;
-      if (sel != null) {
-        fn = sel.Member as Function;
-      }
-      if (fn != null) {
+      if (e is MemberSelectExpr sel && sel.Member is Function fn) {
         Bpl.Expr assertion = !InVerificationScope(fn) ? Bpl.Expr.True : Bpl.Expr.Not(etran.HeightContext(fn));
         builder.Add(Assert(e.tok, assertion,
           "cannot use " + what + " in recursive setting." + hint));
@@ -12264,7 +12266,7 @@ namespace Microsoft.Dafny {
         builder.Add(Bpl.Cmd.SimpleAssign(s.Tok, initHeap, etran.HeapExpr));
       }
       builder.Add(new CommentCmd("TrCallStmt: Before ProcessCallStmt"));
-      ProcessCallStmt(s.Tok, tySubst, GetTypeParams(s.Method), s.Receiver, actualReceiver, s.Method, s.Args, bLhss, lhsTypes, builder, locals, etran);
+      ProcessCallStmt(s.Tok, tySubst, GetTypeParams(s.Method), s.Receiver, actualReceiver, s.Method, s.MethodSelect.AtLabel, s.Args, bLhss, lhsTypes, builder, locals, etran);
       builder.Add(new CommentCmd("TrCallStmt: After ProcessCallStmt"));
       for (int i = 0; i < lhsBuilders.Count; i++) {
         var lhs = s.Lhs[i];
@@ -12315,7 +12317,7 @@ namespace Microsoft.Dafny {
     void ProcessCallStmt(IToken tok,
       Dictionary<TypeParameter, Type> tySubst, List<TypeParameter> tyArgs,
       Expression dafnyReceiver, Bpl.Expr bReceiver,
-      Method method, List<Expression> Args,
+      Method method, Label/*?*/ atLabel, List<Expression> Args,
       List<Bpl.IdentifierExpr> Lhss, List<Type> LhsTypes,
       BoogieStmtListBuilder builder, List<Variable> locals, ExpressionTranslator etran) {
 
@@ -12323,6 +12325,7 @@ namespace Microsoft.Dafny {
       Contract.Requires(dafnyReceiver != null || bReceiver != null);
       Contract.Requires(method != null);
       Contract.Requires(VisibleInScope(method));
+      Contract.Requires(method is TwoStateLemma || atLabel == null);
       Contract.Requires(Args != null);
       Contract.Requires(Lhss != null);
       Contract.Requires(LhsTypes != null);
@@ -12371,7 +12374,7 @@ namespace Microsoft.Dafny {
 
       var ins = new List<Bpl.Expr>();
       if (callee is TwoStateLemma) {
-        ins.Add(etran.Old.HeapExpr);
+        ins.Add(etran.OldAt(atLabel).HeapExpr);
         ins.Add(etran.HeapExpr);
       }
       // Add type arguments
@@ -12460,7 +12463,7 @@ namespace Microsoft.Dafny {
         }
       } else if (method is TwoStateLemma) {
         if (!method.IsStatic) {
-          Bpl.Expr wh = GetWhereClause(receiver.tok, etran.TrExpr(receiver), receiver.Type, etran.Old, ISALLOC, true);
+          Bpl.Expr wh = GetWhereClause(receiver.tok, etran.TrExpr(receiver), receiver.Type, etran.OldAt(atLabel), ISALLOC, true);
           if (wh != null) {
             builder.Add(Assert(receiver.tok, wh, "receiver argument must be allocated in the two-state lemma's previous state"));
           }
@@ -12470,7 +12473,7 @@ namespace Microsoft.Dafny {
           var formal = callee.Ins[i];
           if (formal.IsOld) {
             Expression ee = Args[i];
-            Bpl.Expr wh = GetWhereClause(ee.tok, etran.TrExpr(ee), ee.Type, etran.Old, ISALLOC, true);
+            Bpl.Expr wh = GetWhereClause(ee.tok, etran.TrExpr(ee), ee.Type, etran.OldAt(atLabel), ISALLOC, true);
             if (wh != null) {
               builder.Add(Assert(ee.tok, wh, string.Format("parameter{0} ('{1}') must be allocated in the two-state lemma's previous state",
                 Args.Count == 1 ? "" : " " + i, formal.Name)));
@@ -14815,9 +14818,11 @@ namespace Microsoft.Dafny {
         }
       }
 
-      public ExpressionTranslator OldAt(Label label) {
-        Contract.Requires(label != null);
+      public ExpressionTranslator OldAt(Label/*?*/ label) {
         Contract.Ensures(Contract.Result<ExpressionTranslator>() != null);
+        if (label == null) {
+          return Old;
+        }
         var heapAt = new Bpl.IdentifierExpr(Token.NoToken, "$Heap_at_" + label.AssignUniqueId(translator.CurrentIdGenerator), predef.HeapType);
         return new ExpressionTranslator(translator, predef, heapAt, This, applyLimited_CurrentFunction, layerInterCluster, layerIntraCluster, modifiesFrame, stripLits);
       }
@@ -15400,11 +15405,11 @@ namespace Microsoft.Dafny {
 
         } else if (expr is OldExpr) {
           var e = (OldExpr)expr;
-          return e.AtLabel == null ? Old.TrExpr(e.E) : OldAt(e.AtLabel).TrExpr(e.E);
+          return OldAt(e.AtLabel).TrExpr(e.E);
 
         } else if (expr is UnchangedExpr) {
           var e = (UnchangedExpr)expr;
-          return translator.FrameCondition(e.tok, e.Frame, false, Resolver.FrameExpressionUse.Unchanged, e.AtLabel == null ? Old : OldAt(e.AtLabel), this, this, true);
+          return translator.FrameCondition(e.tok, e.Frame, false, Resolver.FrameExpressionUse.Unchanged, OldAt(e.AtLabel), this, this, true);
 
         } else if (expr is UnaryOpExpr) {
           var e = (UnaryOpExpr)expr;
@@ -16346,7 +16351,7 @@ namespace Microsoft.Dafny {
           args.Add(layerArgument);
         }
         if (e.Function is TwoStateFunction) {
-          args.Add(Old.HeapExpr);
+          args.Add(OldAt(e.AtLabel).HeapExpr);
         }
         if (!omitHeapArgument && (AlwaysUseHeap || e.Function.ReadsHeap)) {
           Contract.Assert(HeapExpr != null);
@@ -17544,7 +17549,7 @@ namespace Microsoft.Dafny {
 
       } else if (expr is OldExpr) {
         var e = (OldExpr)expr;
-        return TrSplitExpr(e.E, splits, position, heightLimit, inlineProtectedFunctions, apply_induction, e.AtLabel == null ? etran.Old : etran.OldAt(e.AtLabel));
+        return TrSplitExpr(e.E, splits, position, heightLimit, inlineProtectedFunctions, apply_induction, etran.OldAt(e.AtLabel));
 
       } else if (expr is FunctionCallExpr && position) {
         var fexp = (FunctionCallExpr)expr;
@@ -18172,7 +18177,7 @@ namespace Microsoft.Dafny {
           FunctionCallExpr e = (FunctionCallExpr)expr;
           Expression receiver = Substitute(e.Receiver);
           List<Expression> newArgs = SubstituteExprList(e.Args);
-          FunctionCallExpr newFce = new FunctionCallExpr(expr.tok, e.Name, receiver, e.OpenParen, newArgs);
+          FunctionCallExpr newFce = new FunctionCallExpr(expr.tok, e.Name, receiver, e.OpenParen, newArgs, e.AtLabel);
           if (e.Function == A) {
             newFce.Function = B;
             newFce.Type = e.Type; // TODO: this may not work with type parameters.
@@ -18365,6 +18370,7 @@ namespace Microsoft.Dafny {
           fseNew.Member = fse.Member;
           fseNew.TypeApplication_AtEnclosingClass = fse.TypeApplication_AtEnclosingClass.ConvertAll(t => Resolver.SubstType(t, typeMap));
           fseNew.TypeApplication_JustMember = fse.TypeApplication_JustMember.ConvertAll(t => Resolver.SubstType(t, typeMap));
+          fseNew.AtLabel = fse.AtLabel;
           newExpr = fseNew;
         } else if (expr is SeqSelectExpr) {
           SeqSelectExpr sse = (SeqSelectExpr)expr;
@@ -18405,7 +18411,7 @@ namespace Microsoft.Dafny {
           if (receiver != e.Receiver || newArgs != e.Args ||
               newTypeApplicationAtEnclosingClass != e.TypeApplication_AtEnclosingClass ||
               newTypeApplicationJustFunction != e.TypeApplication_JustFunction) {
-            FunctionCallExpr newFce = new FunctionCallExpr(expr.tok, e.Name, receiver, e.OpenParen, newArgs);
+            FunctionCallExpr newFce = new FunctionCallExpr(expr.tok, e.Name, receiver, e.OpenParen, newArgs, e.AtLabel);
             newFce.Function = e.Function;  // resolve on the fly (and set newFce.Type below, at end)
             newFce.CoCall = e.CoCall;  // also copy the co-call status
             newFce.CoCallHint = e.CoCallHint;  // and any co-call hint
